Finished QED of SemCompAction to Trace. Ready for next phase. Reorganized sections for future refactoring.

CompileVerifiable.v
@@ -63,14 +63,16 @@ Section Compile.
                     ))
       end.
 
-    Definition compileActions (acts: list (ActionT ty Void)) :=
+  End ReadMap.
+    Definition compileActions (readMap : regMapTy) (acts: list (ActionT ty Void)) :=
       fold_left (fun acc a =>
-                   CompLetFull acc (fun _ writeMap => compileAction a ($$ true)%kami_expr (CompactRegMap (VarRegMap writeMap)))) acts
+                   CompLetFull acc (fun _ writeMap =>
+                                      (CompLetFull (CompRet ($$ WO)%kami_expr (CompactRegMap (VarRegMap writeMap)))
+                                      (fun _ v => @compileAction v _ a ($$ true)%kami_expr (VarRegMap v))))) acts
                 (CompRet ($$ WO)%kami_expr (VarRegMap readMap)).
 
-    Definition compileRules (rules: list RuleT) :=
-      compileActions (map (fun a => snd a ty) rules).
-  End ReadMap.
+    Definition compileRules (readMap : regMapTy) (rules: list RuleT) :=
+      compileActions readMap (map (fun a => snd a ty) rules).
 End Compile.
 
 Section Semantics.
@@ -98,6 +100,12 @@ Section Semantics.
     Proof.
       induction currPriority; simpl; auto; intros.
       inversion H; auto.
+    Qed.
+    
+    Lemma prevPrevRegsTrue' prevUpds:
+      forall prev, PriorityUpds prevUpds prev -> getKindAttr o = getKindAttr prev.
+    Proof.
+      induction 1; eauto.
     Qed.
   End PriorityUpds.
     
@@ -174,320 +182,698 @@ Section Semantics.
       SemCompActionT (@CompLetFull _ _ k a lret cont) regMap_cont (calls_a ++ calls_cont) val_cont.
 End Semantics.
 
-Lemma getKindAttr_fst {A B : Type} {P : B -> Type}  {Q : B -> Type} (l1 : list (A * {x : B & P x})):
-  forall  (l2 : list (A * {x : B & Q x})),
-    getKindAttr l1 = getKindAttr l2 ->
-    (map fst l1) = (map fst l2).
-Proof.
-  induction l1, l2; intros; auto; simpl in *; inv H.
-  erewrite IHl1; eauto.
-Qed.
+Section Properties.
 
-Lemma SemRegExprVals expr :
-  forall o1 o2,
-  SemRegMapExpr expr o1 ->
-  SemRegMapExpr expr o2 ->
-  o1 = o2.
-Proof.
-  induction expr; intros; inv H; inv H0; EqDep_subst; auto;
-    try congruence; specialize (IHexpr _ _ HSemRegMap HSemRegMap0); inv IHexpr; auto.
-Qed.
+  Lemma unifyWO (x : word 0):
+    x = (evalExpr (Const type WO)).
+  Proof.
+    simpl.
+    rewrite (shatter_word_0 x).
+    reflexivity.
+  Qed.
 
-Lemma SemCompActionEquivBexpr (k : Kind) (a : ActionT type k):
-  forall o calls retl expr v' (bexpr1 bexpr2 : Bool @# type),
-    evalExpr bexpr1  = evalExpr bexpr2  ->
-    SemCompActionT (compileAction o a bexpr1 expr) v' calls retl ->
-    SemCompActionT (compileAction o a bexpr2 expr) v' calls retl.
-Proof.
-  induction a; intros; simpl in *; eauto.
-  - inv H1; EqDep_subst; econstructor; eauto.
-  - inv H1; EqDep_subst; econstructor; eauto.
-  - inv H1; EqDep_subst; econstructor; eauto.
-  - inv H1; EqDep_subst; econstructor; eauto.
-  - inv H1; EqDep_subst; econstructor; eauto.
-  - inv H0; simpl in *; EqDep_subst.
-    assert (val_a = evalExpr (Const type WO)) as TMP.
-    {rewrite (shatter_word_0 val_a); auto. }
-    econstructor; eauto.
-    rewrite TMP in HSemCompActionT_a.
-    inv HSemCompActionT_a; EqDep_subst.
-    econstructor; eauto.
-    inv HRegMapWf; destruct regMap_a.
-    split; auto.
-    destruct (bool_dec (evalExpr bexpr2) true).
-    inv H0; EqDep_subst.
-    + econstructor 2; eauto.
-    + congruence.
-    + inv H0; EqDep_subst.
-      * congruence.
-      * econstructor 3; eauto.
-  - inv H1; EqDep_subst.
-    inv HSemCompActionT_cont; EqDep_subst.
-    inv HSemCompActionT_cont0; EqDep_subst.
-    apply Eqdep.EqdepTheory.inj_pair2 in H5; subst; simpl in *.
-    econstructor.
-    + eapply IHa1 with (bexpr1 := (bexpr1 && e)%kami_expr); eauto.
-      simpl; rewrite H0; auto.
-    + econstructor.
-      * eapply IHa2 with (bexpr1 := (bexpr1 && !e)%kami_expr);eauto.
+  Lemma getKindAttr_fst {A B : Type} {P : B -> Type}  {Q : B -> Type} (l1 : list (A * {x : B & P x})):
+    forall  (l2 : list (A * {x : B & Q x})),
+      getKindAttr l1 = getKindAttr l2 ->
+      (map fst l1) = (map fst l2).
+  Proof.
+    induction l1, l2; intros; auto; simpl in *; inv H.
+    erewrite IHl1; eauto.
+  Qed.
+
+  Lemma SemRegExprVals expr :
+    forall o1 o2,
+      SemRegMapExpr expr o1 ->
+      SemRegMapExpr expr o2 ->
+      o1 = o2.
+  Proof.
+    induction expr; intros; inv H; inv H0; EqDep_subst; auto;
+      try congruence; specialize (IHexpr _ _ HSemRegMap HSemRegMap0); inv IHexpr; auto.
+  Qed.
+
+  Lemma SemCompActionEquivBexpr (k : Kind) (a : ActionT type k):
+    forall o calls retl expr v' (bexpr1 bexpr2 : Bool @# type),
+      evalExpr bexpr1  = evalExpr bexpr2  ->
+      SemCompActionT (compileAction o a bexpr1 expr) v' calls retl ->
+      SemCompActionT (compileAction o a bexpr2 expr) v' calls retl.
+  Proof.
+    induction a; intros; simpl in *; eauto.
+    - inv H1; EqDep_subst; econstructor; eauto.
+    - inv H1; EqDep_subst; econstructor; eauto.
+    - inv H1; EqDep_subst; econstructor; eauto.
+    - inv H1; EqDep_subst; econstructor; eauto.
+    - inv H1; EqDep_subst; econstructor; eauto.
+    - inv H0; simpl in *; EqDep_subst.
+      econstructor; eauto.
+      rewrite (unifyWO val_a) in HSemCompActionT_a.
+      inv HSemCompActionT_a; EqDep_subst.
+      econstructor; eauto.
+      inv HRegMapWf; destruct regMap_a.
+      split; auto.
+      destruct (bool_dec (evalExpr bexpr2) true).
+      inv H0; EqDep_subst.
+      + econstructor 2; eauto.
+      + congruence.
+      + inv H0; EqDep_subst.
+        * congruence.
+        * econstructor 3; eauto.
+    - inv H1; EqDep_subst.
+      inv HSemCompActionT_cont; EqDep_subst.
+      inv HSemCompActionT_cont0; simpl in *; EqDep_subst.
+      econstructor.
+      + eapply IHa1 with (bexpr1 := (bexpr1 && e)%kami_expr); eauto.
         simpl; rewrite H0; auto.
-      * econstructor; simpl.
-        eapply H; eauto.
-  - inv H0; EqDep_subst.
-    econstructor; eauto.
-Qed.
+      + econstructor.
+        * eapply IHa2 with (bexpr1 := (bexpr1 && !e)%kami_expr);eauto.
+          simpl; rewrite H0; auto.
+        * econstructor; simpl.
+          eapply H; eauto.
+    - inv H0; EqDep_subst.
+      econstructor; eauto.
+  Qed.
 
-Lemma predFalse_UpdsNil k a:
-  forall (bexpr: Bool @# type) o regMap1 regMap2 calls val
-         (HNbexpr : evalExpr bexpr = false) rexpr (HRegMap : SemRegMapExpr rexpr regMap1),
-    @SemCompActionT k (compileAction (o, nil) a bexpr rexpr) regMap2 calls val ->
-    regMap1 = regMap2 /\ calls = nil.
-Proof.
-  induction a; intros.
-  - inv H0; EqDep_subst;[congruence|eauto].
-  - inv H0; EqDep_subst; eauto.
-  - inv H0; EqDep_subst; eauto.
-    specialize (IHa _ _ _ _ _ _ HNbexpr _ HRegMap HSemCompActionT_a); dest.
-    rewrite H0 in HRegMap.
-    assert (SemRegMapExpr (VarRegMap type regMap_a) regMap_a);[constructor|].
-    specialize (H _ _ _ _ _ _ _ HNbexpr _ H2 HSemCompActionT_cont); dest.
-    split; subst; auto.
-  - inv H0; EqDep_subst; eauto.
-  - inv H0; EqDep_subst; eauto.
-  - inv H; simpl in *; EqDep_subst; eauto.
-    assert (val_a = evalExpr (Const type WO)) as TMP.
-    {rewrite (shatter_word_0 val_a); auto. }
-    rewrite TMP in HSemCompActionT_a.
-    inv HSemCompActionT_a; EqDep_subst.
-    inv HRegMapWf; inv H; EqDep_subst;[congruence|].
-    assert (SemRegMapExpr (VarRegMap type (old, upds)) (old, upds));[constructor|].
-    specialize (IHa _ _ _ _ _ _ HNbexpr _ H HSemCompActionT_cont); dest.
-    rewrite (SemRegExprVals HRegMap HSemRegMap); auto.
-  - simpl in *; inv H0; EqDep_subst.
-    inv HSemCompActionT_cont; EqDep_subst.
-    inv HSemCompActionT_cont0; EqDep_subst.
-    apply Eqdep.EqdepTheory.inj_pair2 in H4; subst; simpl in *.
-    assert (forall b, (evalExpr (bexpr && b)%kami_expr = false)).
-    { intros; simpl; rewrite HNbexpr; auto. }
-    specialize (IHa1 _ _ _ _ _ _ (H0 e) _ HRegMap HSemCompActionT_a); dest.
-    assert (SemRegMapExpr (VarRegMap type regMap_a) regMap1) as P0.
-    { rewrite H1; constructor. }
-    specialize (IHa2 _ _ _ _ _ _ (H0 (!e)%kami_expr) _ P0 HSemCompActionT_a0); dest.
-    assert (SemRegMapExpr (VarRegMap type regMap_a0) regMap1) as P1.
-    { rewrite <- H3. constructor. }
-    specialize (H _ _ _ _ _ _ _ HNbexpr _ P1 HSemCompActionT); dest.
-    subst; auto.
-  - inv H; EqDep_subst; eauto.
-  - inv H; EqDep_subst.
-    inv HRegMapWf.
-    specialize (SemRegExprVals HRegMap H) as P0; auto.
-Qed.
+  Lemma predFalse_UpdsNil k a:
+    forall (bexpr: Bool @# type) o u regMap1 regMap2 calls val
+           (HNbexpr : evalExpr bexpr = false) rexpr (HRegMap : SemRegMapExpr rexpr regMap1),
+      @SemCompActionT k (compileAction (o, u) a bexpr rexpr) regMap2 calls val ->
+      regMap1 = regMap2 /\ calls = nil.
+  Proof.
+    induction a; intros.
+    - inv H0; EqDep_subst;[congruence|eauto].
+    - inv H0; EqDep_subst; eauto.
+    - inv H0; EqDep_subst; eauto.
+      specialize (IHa _ _ _ _ _ _ _ HNbexpr _ HRegMap HSemCompActionT_a); dest.
+      rewrite H0 in HRegMap.
+      assert (SemRegMapExpr (VarRegMap type regMap_a) regMap_a);[constructor|].
+      specialize (H _ _ _ _ _ _ _ _ HNbexpr _ H2 HSemCompActionT_cont); dest.
+      split; subst; auto.
+    - inv H0; EqDep_subst; eauto.
+    - inv H0; EqDep_subst; eauto.
+    - inv H; simpl in *; EqDep_subst; eauto.
+      rewrite (unifyWO val_a) in HSemCompActionT_a.
+      inv HSemCompActionT_a; EqDep_subst.
+      inv HRegMapWf; inv H; EqDep_subst;[congruence|].
+      assert (SemRegMapExpr (VarRegMap type (old, upds)) (old, upds));[constructor|].
+      specialize (IHa _ _ _ _ _ _ _ HNbexpr _ H HSemCompActionT_cont); dest.
+      rewrite (SemRegExprVals HRegMap HSemRegMap); auto.
+    - simpl in *; inv H0; EqDep_subst.
+      inv HSemCompActionT_cont; EqDep_subst.
+      inv HSemCompActionT_cont0; EqDep_subst.
+      apply Eqdep.EqdepTheory.inj_pair2 in H4; subst; simpl in *.
+      assert (forall b, (evalExpr (bexpr && b)%kami_expr = false)).
+      { intros; simpl; rewrite HNbexpr; auto. }
+      specialize (IHa1 _ _ _ _ _ _ _ (H0 e) _ HRegMap HSemCompActionT_a); dest.
+      assert (SemRegMapExpr (VarRegMap type regMap_a) regMap1) as P0.
+      { rewrite H1; constructor. }
+      specialize (IHa2 _ _ _ _ _ _ _ (H0 (!e)%kami_expr) _ P0 HSemCompActionT_a0); dest.
+      assert (SemRegMapExpr (VarRegMap type regMap_a0) regMap1) as P1.
+      { rewrite <- H3. constructor. }
+      specialize (H _ _ _ _ _ _ _ _ HNbexpr _ P1 HSemCompActionT); dest.
+      subst; auto.
+    - inv H; EqDep_subst; eauto.
+    - inv H; EqDep_subst.
+      inv HRegMapWf.
+      specialize (SemRegExprVals HRegMap H) as P0; auto.
+  Qed.
 
-Lemma UpdRegs_same_nil o :
-  UpdRegs (nil::nil) o o.
-Proof.
-  unfold UpdRegs.
-  repeat split; auto.
-  intros.
-  right; unfold not; split; intros; dest; auto.
-  destruct H0; subst; auto.
-Qed.
+  Lemma UpdRegs_same_nil o :
+    UpdRegs (nil::nil) o o.
+  Proof.
+    unfold UpdRegs.
+    repeat split; auto.
+    intros.
+    right; unfold not; split; intros; dest; auto.
+    destruct H0; subst; auto.
+  Qed.
 
-Lemma NoDup_app_split {A : Type} (l l' : list A) :
-  NoDup (l++l') ->
-  forall a,
-    In a l ->
-    ~ In a l'.
-Proof.
-  induction l'; repeat intro;[inv H1|].
-  specialize (NoDup_remove _ _ _ H) as P0; dest.
-  inv H1; apply H3; rewrite in_app_iff; auto.
-  exfalso; eapply IHl'; eauto.
-Qed.
+  Lemma NoDup_app_split {A : Type} (l l' : list A) :
+    NoDup (l++l') ->
+    forall a,
+      In a l ->
+      ~ In a l'.
+  Proof.
+    induction l'; repeat intro;[inv H1|].
+    specialize (NoDup_remove _ _ _ H) as P0; dest.
+    inv H1; apply H3; rewrite in_app_iff; auto.
+    exfalso; eapply IHl'; eauto.
+  Qed.
 
-Lemma EquivActions k a:
-  forall
-    writeMap o old upds
-    (HConsistent : getKindAttr o = getKindAttr old)
-    (WfMap : WfRegMapExpr writeMap (old, upds)),
-  forall calls retl upds',
-    @SemCompActionT k (compileAction (o, nil) a (Const type true) writeMap) upds' calls retl ->
-    (forall u, In u (snd upds') -> NoDup (map fst u) /\ SubList (getKindAttr u) (getKindAttr old)) /\
-    exists newRegs readRegs,
-      upds' = (old, match newRegs with
-                    |nil => upds
-                    |_ :: _ => (hd nil upds ++ newRegs) :: tl upds
-                    end) /\
-      SemAction o a readRegs newRegs calls retl.
-Proof.
-  induction a; subst; intros; simpl in *.
-  - inv H0; EqDep_subst;[|discriminate].
-    specialize (H _ _ _ _ _ HConsistent WfMap _ _ _ HSemCompActionT); dest; split; auto.
-    exists x, x0; split; auto.
-    econstructor; eauto.
-  - inv H0; EqDep_subst.
-    specialize (H _ _ _ _ _ HConsistent WfMap _ _ _ HSemCompActionT); dest; split; auto.
-    exists x, x0; split; auto.
-    econstructor; eauto.
-  - inv H0; EqDep_subst.
-    specialize (IHa _ _ _ _ HConsistent WfMap _ _ _ HSemCompActionT_a); dest.
-    assert (WfRegMapExpr (VarRegMap type regMap_a) regMap_a) as WfMap0.
-    { unfold WfRegMapExpr; split;[econstructor|].
-      destruct regMap_a; inv H1; intros.
-      apply (H0 _ H1).
-    }
-    rewrite H1 in *.
-    specialize (H _ _ _ _ _ HConsistent WfMap0 _ _ _ HSemCompActionT_cont); dest.
-    split; auto.
-    exists (x++x1), (x0++x2); split.
-    + destruct x1; simpl in *; auto.
-      * rewrite app_nil_r; assumption.
-      * destruct x; simpl in *; auto.
-        rewrite app_comm_cons, app_assoc; assumption.
-    + econstructor; eauto.
-      rewrite H3 in H; simpl in *.
-      clear - H.
-      destruct x, x1; eauto using DisjKey_nil_r, DisjKey_nil_l; simpl in *.
-      specialize (H _ (or_introl _ eq_refl)); simpl in *; dest.
-      repeat rewrite map_app in H.
-      intro k.
-      destruct (In_dec string_dec k (map fst (p0::x1))); auto.
-      left; intro.
-      destruct (NoDup_app_Disj string_dec _ _ H k); auto.
-      apply H2; rewrite in_app_iff; right; auto.
-  - inv H0; EqDep_subst.
-    specialize (H _ _ _ _ _ HConsistent WfMap _ _ _ HSemCompActionT); dest; split; auto.
-    exists x, x0; split; auto.
-    econstructor; eauto.
-  - inv H0; EqDep_subst.
-    specialize (H _ _ _ _ _ HConsistent WfMap _ _ _ HSemCompActionT); dest; split; auto.
-    exists x, ((r, existT _ k regVal) :: x0).
-    split; auto.
-    econstructor; eauto.
-    inv HReadMap; inv HUpdatedRegs; auto.
-    discriminate.
-  - inv H; simpl in *; EqDep_subst.
-    assert (val_a = evalExpr (Const type WO)) as TMP.
-    {rewrite (shatter_word_0 val_a); auto. }
-    rewrite TMP in HSemCompActionT_a.
-    inv HSemCompActionT_a; EqDep_subst.
-    destruct HRegMapWf, WfMap, regMap_a.
-    inv H;[|discriminate]; EqDep_subst.
-    specialize (SemRegExprVals H1 HSemRegMap) as P0; inv P0.
-    assert (WfRegMapExpr (VarRegMap type (r0, (hd nil upds0 ++ (r, existT (fullType type) k (evalExpr e)) :: nil) :: tl upds0))
-                         (r0, (hd nil upds0 ++ (r, existT (fullType type) k (evalExpr e)) :: nil) :: tl upds0)) as WfMap0.
-    { split; auto. constructor. }
-    specialize (IHa _ _ _ _ HConsistent WfMap0 _ _ _ HSemCompActionT_cont);
-      dest; simpl in *; split; auto.
-    exists ((r, existT (fullType type) k (evalExpr e)) :: nil ++ x), x0; split.
-    + destruct x; simpl in *; auto.
-      rewrite <- app_assoc in H3. rewrite <-app_comm_cons in H3.
-      simpl in H3; auto.
-    + rewrite H3 in H; simpl in *; destruct x; econstructor; eauto; simpl in *; specialize (H _ (or_introl _ eq_refl)); dest.
-      * rewrite map_app, <-HConsistent in H6; simpl in *.
-        apply (H6 (r, k)).
-        rewrite in_app_iff; right; left; reflexivity.
-      * repeat intro; inv H7.
-      * rewrite map_app, <-HConsistent in H6; simpl in *.
-        apply (H6 (r, k)).
-        rewrite map_app; repeat rewrite in_app_iff; simpl; auto.
-      * repeat intro.
-        repeat rewrite map_app in H; simpl in *.
-        destruct H7; subst; destruct (NoDup_app_Disj string_dec _ _ H r) as [P0|P0]; apply P0.
-        -- rewrite in_app_iff; simpl; auto.
-        -- simpl; auto.
-        -- rewrite in_app_iff; simpl; auto.
-        -- simpl; right; rewrite in_map_iff.
-           exists (r, v); simpl; auto.
-  - inv H0; EqDep_subst.
-    inv HSemCompActionT_cont; EqDep_subst.
-    inv HSemCompActionT_cont0; EqDep_subst.
-    remember (evalExpr e) as P0.
-    apply Eqdep.EqdepTheory.inj_pair2 in H4.
-    rewrite H4 in *.
-    clear H4; simpl in *.
-    assert (forall bexpr, (evalExpr (Const type true && bexpr)%kami_expr = evalExpr bexpr)) as P1.
-    { intro; simpl; auto. }
-    specialize (SemCompActionEquivBexpr _ _ _ _ _ (P1 e) HSemCompActionT_a) as P2.
-    specialize (SemCompActionEquivBexpr _ _ _ _ _ (P1 (!e)%kami_expr) HSemCompActionT_a0) as P3.
-    destruct P0; simpl in *.
-    + assert (evalExpr e = evalExpr (Const type true)) as P4; simpl; auto.
-      assert (evalExpr (!e)%kami_expr = false) as P5.
-      { simpl; rewrite <- HeqP0; auto. }
-      specialize (SemCompActionEquivBexpr _ _ _ _ _ P4 P2) as P6.
-      specialize (IHa1 _ _ _ _ HConsistent WfMap _ _ _ P6); dest.
-      rewrite <- HeqP0 in HSemCompActionT.
-      destruct (predFalse_UpdsNil _ _ _ P5 (SemVarRegMap regMap_a) P3).
-      assert (WfRegMapExpr (VarRegMap type regMap_a0) regMap_a0) as P7.
-      { unfold WfRegMapExpr; split; [constructor|]. subst; eauto. }
-      rewrite <- H3 in P7 at 2.
-      rewrite H1 in P7.
-      specialize (H _ _ _ _ _ HConsistent P7 _ _ _ HSemCompActionT); dest.
-      split; auto.
-      exists (x++x1), (x0++x2).
-      destruct x; simpl; split; auto.
-      * rewrite H4.
-        econstructor; eauto.
-        apply DisjKey_nil_l.
-      * destruct x1;[rewrite app_nil_r|]; simpl in *; auto.
-        rewrite <-app_assoc, <-app_comm_cons in H5; assumption.
-      * rewrite H4; simpl.
-        econstructor; eauto.
-        rewrite H5 in H; simpl in *.
-        clear - H.
-        destruct x1; simpl in *; [apply DisjKey_nil_r|].
-        specialize (H _ (or_introl _ (eq_refl))); dest.
-        rewrite map_app in H.
-        intro.
-        destruct (NoDup_app_Disj string_dec _ _ H k); auto.
-        left; intro; apply H1.
-        rewrite map_app, in_app_iff; auto.
-    + assert (evalExpr (!e)%kami_expr = evalExpr (Const type true)) as P4.
-      { simpl; rewrite <- HeqP0; auto. }
-      specialize (SemCompActionEquivBexpr _ _ _ _ _ P4 P3) as P6.
-      remember WfMap as WfMap0.
-      inv WfMap0.
-      destruct (predFalse_UpdsNil _ _ _ (eq_sym HeqP0) H0 P2).
-      assert (WfRegMapExpr (VarRegMap type regMap_a) (old, upds)) as WfMap0.
-      { rewrite <- H2.
-        clear - WfMap.
-        unfold WfRegMapExpr in *; dest; repeat split;[constructor| |]; eapply H0; eauto.
+  Lemma PriorityUpds_Equiv old upds new
+        (HNoDupOld : NoDup (map fst old))
+        (HNoDupUpds : forall u, In u upds -> NoDup (map fst u)) :
+    PriorityUpds old upds new ->
+    forall new',
+      PriorityUpds old upds new' ->
+      SubList new new'.
+  Proof.
+    induction 1; intros.
+    - inv H.
+      + apply SubList_refl.
+      + discriminate.
+    - subst.
+      inv H0; inv HFullU.
+      repeat intro.
+      destruct x.
+      specialize (Hcurr _ _ H0).
+      specialize (getKindAttr_map_fst _ _ currRegsTCurr0) as P0.
+      specialize (getKindAttr_map_fst _ _ currRegsTCurr) as P1.
+      assert (In s (map fst new')).
+      { rewrite <- P0, P1, in_map_iff. exists (s, s0); split; auto. }
+      rewrite in_map_iff in H1; dest.
+      destruct x; simpl in *; subst.
+      specialize (Hcurr0 _ _ H2).
+      specialize (HNoDupUpds _ (or_introl _ (eq_refl))) as P3.
+      destruct Hcurr, Hcurr0; dest.
+      + rewrite <-(KeyMatching3 _ _ _ P3 H3 H1 eq_refl).
+        assumption.
+      + exfalso; apply H3.
+        rewrite in_map_iff.
+        exists (s, s0); split; auto.
+      + exfalso; apply H1.
+        rewrite in_map_iff.
+        exists (s, s2); split; auto.
+      + assert (forall u,  In u prevUpds0 -> NoDup (map fst u)) as P4; eauto.
+        specialize (IHPriorityUpds P4 _ prevCorrect _ H5).
+        rewrite (getKindAttr_map_fst _ _ (prevPrevRegsTrue' prevCorrect)) in HNoDupOld.
+        rewrite (KeyMatching3 _ _ _ HNoDupOld H4 IHPriorityUpds eq_refl) in *.
+        assumption.
+  Qed.
+
+  Lemma EquivActions k a:
+    forall
+      writeMap o old upds oInit uInit
+      (HoInitNoDups : NoDup (map fst oInit))
+      (HuInitNoDups : forall u, In u uInit -> NoDup (map fst u))
+      (HPriorityUpds : PriorityUpds oInit uInit o)
+      (HConsistent : getKindAttr o = getKindAttr old)
+      (WfMap : WfRegMapExpr writeMap (old, upds)),
+    forall calls retl upds',
+      @SemCompActionT k (compileAction (oInit, uInit) a (Const type true) writeMap) upds' calls retl ->
+      (forall u, In u (snd upds') -> NoDup (map fst u) /\ SubList (getKindAttr u) (getKindAttr old)) /\
+      exists newRegs readRegs,
+        upds' = (old, match newRegs with
+                      |nil => upds
+                      |_ :: _ => (hd nil upds ++ newRegs) :: tl upds
+                      end) /\
+        SemAction o a readRegs newRegs calls retl.
+  Proof.
+    induction a; subst; intros; simpl in *.
+    - inv H0; EqDep_subst;[|discriminate].
+      specialize (H _ _ _ _ _ _ _ HoInitNoDups HuInitNoDups HPriorityUpds HConsistent WfMap _ _ _ HSemCompActionT); dest; split; auto.
+      exists x, x0; split; auto.
+      econstructor; eauto.
+    - inv H0; EqDep_subst.
+      specialize (H _ _ _ _ _ _ _ HoInitNoDups HuInitNoDups HPriorityUpds HConsistent WfMap _ _ _ HSemCompActionT); dest; split; auto.
+      exists x, x0; split; auto.
+      econstructor; eauto.
+    - inv H0; EqDep_subst.
+      specialize (IHa _ _ _ _ _ _ HoInitNoDups HuInitNoDups HPriorityUpds HConsistent WfMap _ _ _ HSemCompActionT_a); dest.
+      assert (WfRegMapExpr (VarRegMap type regMap_a) regMap_a) as WfMap0.
+      { unfold WfRegMapExpr; split;[econstructor|].
+        destruct regMap_a; inv H1; intros.
+        apply (H0 _ H1).
       }
-      specialize (IHa2 _ _ _ _ HConsistent WfMap0 _ _ _ P6); dest.
-      rewrite <- HeqP0 in HSemCompActionT.
-      assert (WfRegMapExpr (VarRegMap type regMap_a0) regMap_a0) as P7.
-      { unfold WfRegMapExpr; split; [constructor|]. subst; eauto. }
-      rewrite  H5 in P7 at 2.
-      specialize (H _ _ _ _ _ HConsistent P7 _ _ _ HSemCompActionT); dest.
+      rewrite H1 in *.
+      specialize (H _ _ _ _ _ _ _ HoInitNoDups HuInitNoDups HPriorityUpds HConsistent WfMap0 _ _ _ HSemCompActionT_cont); dest.
       split; auto.
-      exists (x++x1), (x0++x2).
-      destruct x; simpl; split; auto.
-      * rewrite H3; simpl.
-        econstructor 8; eauto.
-        apply DisjKey_nil_l.
-      * destruct x1;[rewrite app_nil_r|]; simpl in *; auto.
-        rewrite <-app_assoc, <-app_comm_cons in H7; assumption.
-      * rewrite H3; simpl.
-        econstructor 8; eauto.
-        rewrite H7 in H; simpl in *.
+      exists (x++x1), (x0++x2); split.
+      + destruct x1; simpl in *; auto.
+        * rewrite app_nil_r; assumption.
+        * destruct x; simpl in *; auto.
+          rewrite app_comm_cons, app_assoc; assumption.
+      + econstructor; eauto.
+        rewrite H3 in H; simpl in *.
         clear - H.
-        destruct x1; simpl in *; [apply DisjKey_nil_r|].
-        specialize (H _ (or_introl _ (eq_refl))); dest.
-        rewrite map_app in H.
-        intro.
+        destruct x, x1; eauto using DisjKey_nil_r, DisjKey_nil_l; simpl in *.
+        specialize (H _ (or_introl _ eq_refl)); simpl in *; dest.
+        repeat rewrite map_app in H.
+        intro k.
+        destruct (In_dec string_dec k (map fst (p0::x1))); auto.
+        left; intro.
         destruct (NoDup_app_Disj string_dec _ _ H k); auto.
-        left; intro; apply H1.
-        rewrite map_app, in_app_iff; auto.
-  - inv H; EqDep_subst.
-    specialize (IHa _ _ _ _ HConsistent WfMap _ _ _ HSemCompActionT); dest; split; auto.
-    exists x, x0.
-    split; auto.
-    econstructor; eauto.
-  - inv H; EqDep_subst.
-    inv WfMap; inv HRegMapWf.
-    specialize (SemRegExprVals H H1) as TMP; subst; simpl in *.
-    split; auto.
-    exists nil, nil.
-    split; auto.
-    constructor; auto.
-Qed.
+        apply H2; rewrite in_app_iff; right; auto.
+    - inv H0; EqDep_subst.
+      specialize (H _ _ _ _ _ _ _ HoInitNoDups HuInitNoDups HPriorityUpds HConsistent WfMap _ _ _ HSemCompActionT); dest; split; auto.
+      exists x, x0; split; auto.
+      econstructor; eauto.
+    - inv H0; EqDep_subst.
+      specialize (H _ _ _ _ _ _ _ HoInitNoDups HuInitNoDups HPriorityUpds HConsistent WfMap _ _ _ HSemCompActionT); dest; split; auto.
+      exists x, ((r, existT _ k regVal) :: x0).
+      split; auto.
+      econstructor; eauto.
+      inv HReadMap.
+      apply (PriorityUpds_Equiv HoInitNoDups HuInitNoDups HUpdatedRegs HPriorityUpds); auto.
+    - inv H; simpl in *; EqDep_subst.
+      rewrite (unifyWO val_a) in HSemCompActionT_a.
+      inv HSemCompActionT_a; EqDep_subst.
+      destruct HRegMapWf, WfMap, regMap_a.
+      inv H;[|discriminate]; EqDep_subst.
+      specialize (SemRegExprVals H1 HSemRegMap) as P0; inv P0.
+      assert (WfRegMapExpr (VarRegMap type (r0, (hd nil upds0 ++ (r, existT (fullType type) k (evalExpr e)) :: nil) :: tl upds0))
+                           (r0, (hd nil upds0 ++ (r, existT (fullType type) k (evalExpr e)) :: nil) :: tl upds0)) as WfMap0.
+      { split; auto. constructor. }
+      specialize (IHa _ _ _ _ _ _ HoInitNoDups HuInitNoDups HPriorityUpds HConsistent WfMap0 _ _ _ HSemCompActionT_cont);
+        dest; simpl in *; split; auto.
+      exists ((r, existT (fullType type) k (evalExpr e)) :: nil ++ x), x0; split.
+      + destruct x; simpl in *; auto.
+        rewrite <- app_assoc in H3. rewrite <-app_comm_cons in H3.
+        simpl in H3; auto.
+      + rewrite H3 in H; simpl in *; destruct x; econstructor; eauto; simpl in *; specialize (H _ (or_introl _ eq_refl)); dest.
+        * rewrite map_app, <-HConsistent in H6; simpl in *.
+          apply (H6 (r, k)).
+          rewrite in_app_iff; right; left; reflexivity.
+        * repeat intro; inv H7.
+        * rewrite map_app, <-HConsistent in H6; simpl in *.
+          apply (H6 (r, k)).
+          rewrite map_app; repeat rewrite in_app_iff; simpl; auto.
+        * repeat intro.
+          repeat rewrite map_app in H; simpl in *.
+          destruct H7; subst; destruct (NoDup_app_Disj string_dec _ _ H r) as [P0|P0]; apply P0.
+          -- rewrite in_app_iff; simpl; auto.
+          -- simpl; auto.
+          -- rewrite in_app_iff; simpl; auto.
+          -- simpl; right; rewrite in_map_iff.
+             exists (r, v); simpl; auto.
+    - inv H0; EqDep_subst.
+      inv HSemCompActionT_cont; EqDep_subst.
+      inv HSemCompActionT_cont0; EqDep_subst.
+      remember (evalExpr e) as P0.
+      apply Eqdep.EqdepTheory.inj_pair2 in H4.
+      rewrite H4 in *.
+      clear H4; simpl in *.
+      assert (forall bexpr, (evalExpr (Const type true && bexpr)%kami_expr = evalExpr bexpr)) as P1.
+      { intro; simpl; auto. }
+      specialize (SemCompActionEquivBexpr _ _ _ _ _ (P1 e) HSemCompActionT_a) as P2.
+      specialize (SemCompActionEquivBexpr _ _ _ _ _ (P1 (!e)%kami_expr) HSemCompActionT_a0) as P3.
+      destruct P0; simpl in *.
+      + assert (evalExpr e = evalExpr (Const type true)) as P4; simpl; auto.
+        assert (evalExpr (!e)%kami_expr = false) as P5.
+        { simpl; rewrite <- HeqP0; auto. }
+        specialize (SemCompActionEquivBexpr _ _ _ _ _ P4 P2) as P6.
+        specialize (IHa1 _ _ _ _ _ _ HoInitNoDups HuInitNoDups HPriorityUpds HConsistent WfMap _ _ _ P6); dest.
+        rewrite <- HeqP0 in HSemCompActionT.
+        destruct (predFalse_UpdsNil _ _ _ _ P5 (SemVarRegMap regMap_a) P3).
+        assert (WfRegMapExpr (VarRegMap type regMap_a0) regMap_a0) as P7.
+        { unfold WfRegMapExpr; split; [constructor|]. subst; eauto. }
+        rewrite <- H3 in P7 at 2.
+        rewrite H1 in P7.
+        specialize (H _ _ _ _ _ _ _ HoInitNoDups HuInitNoDups HPriorityUpds HConsistent P7 _ _ _ HSemCompActionT); dest.
+        split; auto.
+        exists (x++x1), (x0++x2).
+        destruct x; simpl; split; auto.
+        * rewrite H4.
+          econstructor; eauto.
+          apply DisjKey_nil_l.
+        * destruct x1;[rewrite app_nil_r|]; simpl in *; auto.
+          rewrite <-app_assoc, <-app_comm_cons in H5; assumption.
+        * rewrite H4; simpl.
+          econstructor; eauto.
+          rewrite H5 in H; simpl in *.
+          clear - H.
+          destruct x1; simpl in *; [apply DisjKey_nil_r|].
+          specialize (H _ (or_introl _ (eq_refl))); dest.
+          rewrite map_app in H.
+          intro.
+          destruct (NoDup_app_Disj string_dec _ _ H k); auto.
+          left; intro; apply H1.
+          rewrite map_app, in_app_iff; auto.
+      + assert (evalExpr (!e)%kami_expr = evalExpr (Const type true)) as P4.
+        { simpl; rewrite <- HeqP0; auto. }
+        specialize (SemCompActionEquivBexpr _ _ _ _ _ P4 P3) as P6.
+        remember WfMap as WfMap0.
+        inv WfMap0.
+        destruct (predFalse_UpdsNil _ _ _ _ (eq_sym HeqP0) H0 P2).
+        assert (WfRegMapExpr (VarRegMap type regMap_a) (old, upds)) as WfMap0.
+        { rewrite <- H2.
+          clear - WfMap.
+          unfold WfRegMapExpr in *; dest; repeat split;[constructor| |]; eapply H0; eauto.
+        }
+        specialize (IHa2 _ _ _ _ _ _ HoInitNoDups HuInitNoDups HPriorityUpds HConsistent WfMap0 _ _ _ P6); dest.
+        rewrite <- HeqP0 in HSemCompActionT.
+        assert (WfRegMapExpr (VarRegMap type regMap_a0) regMap_a0) as P7.
+        { unfold WfRegMapExpr; split; [constructor|]. subst; eauto. }
+        rewrite  H5 in P7 at 2.
+        specialize (H _ _ _ _ _ _ _ HoInitNoDups HuInitNoDups HPriorityUpds HConsistent P7 _ _ _ HSemCompActionT); dest.
+        split; auto.
+        exists (x++x1), (x0++x2).
+        destruct x; simpl; split; auto.
+        * rewrite H3; simpl.
+          econstructor 8; eauto.
+          apply DisjKey_nil_l.
+        * destruct x1;[rewrite app_nil_r|]; simpl in *; auto.
+          rewrite <-app_assoc, <-app_comm_cons in H7; assumption.
+        * rewrite H3; simpl.
+          econstructor 8; eauto.
+          rewrite H7 in H; simpl in *.
+          clear - H.
+          destruct x1; simpl in *; [apply DisjKey_nil_r|].
+          specialize (H _ (or_introl _ (eq_refl))); dest.
+          rewrite map_app in H.
+          intro.
+          destruct (NoDup_app_Disj string_dec _ _ H k); auto.
+          left; intro; apply H1.
+          rewrite map_app, in_app_iff; auto.
+    - inv H; EqDep_subst.
+      specialize (IHa _ _ _ _ _ _ HoInitNoDups HuInitNoDups HPriorityUpds HConsistent WfMap _ _ _ HSemCompActionT); dest; split; auto.
+      exists x, x0.
+      split; auto.
+      econstructor; eauto.
+    - inv H; EqDep_subst.
+      inv WfMap; inv HRegMapWf.
+      specialize (SemRegExprVals H H1) as TMP; subst; simpl in *.
+      split; auto.
+      exists nil, nil.
+      split; auto.
+      constructor; auto.
+  Qed.
+
+
+  Lemma SameOldAction (k : Kind) (a : ActionT type k) :
+    forall oInit uInit writeMap old upds wOld wUpds calls retl bexpr
+           (HSemRegMap : SemRegMapExpr writeMap (wOld, wUpds)),
+      @SemCompActionT k (compileAction (oInit, uInit) a bexpr writeMap) (old, upds) calls retl ->
+      wOld = old.
+  Proof.
+    induction a; intros; simpl in *.
+    - inv H0; EqDep_subst; simpl in *; eapply H; eauto.
+    - inv H0; EqDep_subst; simpl in *.
+      eapply H; eauto.
+    - inv H0; EqDep_subst; simpl in *.
+      assert (SemRegMapExpr (VarRegMap type regMap_a) regMap_a) as P0.
+      { constructor. }
+      destruct regMap_a.
+      specialize (H _ _ _ _ _ _ _ _ _ _ _ P0 HSemCompActionT_cont); subst.
+      specialize (IHa _ _ _ _ _ _ _ _ _ _ HSemRegMap HSemCompActionT_a); assumption.
+    - inv H0; EqDep_subst; simpl in *.
+      eapply H; eauto.
+    - inv H0; EqDep_subst; simpl in *.
+      eapply H; eauto.
+    - inv H; simpl in *; EqDep_subst.
+      rewrite (unifyWO val_a) in HSemCompActionT_a.
+      inv HSemCompActionT_a; EqDep_subst.
+      destruct regMap_a; unfold WfRegMapExpr in *; dest.
+      inv H; EqDep_subst.
+      + assert (SemRegMapExpr (VarRegMap type (r0, (hd nil upds0 ++ (r, existT (fullType type) k (evalExpr e)) :: nil) :: tl upds0))
+                              (r0, (hd nil upds0 ++ (r, existT (fullType type) k (evalExpr e)) :: nil) :: tl upds0)) as P0.
+        { constructor. }
+        specialize (IHa _ _ _ _ _ _ _ _ _ _ P0 HSemCompActionT_cont).
+        specialize (SemRegExprVals HSemRegMap HSemRegMap0) as TMP; inv TMP.
+        reflexivity.
+      + specialize (IHa _ _ _ _ _ _ _ _ _ _ (SemVarRegMap _) HSemCompActionT_cont).
+        specialize (SemRegExprVals HSemRegMap HSemRegMap0) as TMP; inv TMP.
+        reflexivity.
+    - inv H0; EqDep_subst; simpl in *.
+      inv HSemCompActionT_cont; EqDep_subst.
+      inv HSemCompActionT_cont0; simpl in *; EqDep_subst.
+      destruct regMap_a, regMap_a0.
+      specialize (H _ _ _ _ _ _ _ _ _ _ _ (SemVarRegMap _) HSemCompActionT).
+      simpl in *.
+      specialize (IHa1 _ _ _ _ _ _ _ _ _ _ HSemRegMap HSemCompActionT_a).
+      specialize (IHa2 _ _ _ _ _ _ _ _ _ _ (SemVarRegMap _) HSemCompActionT_a0).
+      subst; reflexivity.
+    - inv H; EqDep_subst; simpl in *.
+      eapply IHa; eauto.
+    - inv H; EqDep_subst.
+      unfold WfRegMapExpr in *; dest.
+      specialize (SemRegExprVals H HSemRegMap) as TMP; inv TMP.
+      reflexivity.
+  Qed.
+
+  Lemma SameOldActions o:
+    forall la old upds calls retl,
+      @SemCompActionT Void (compileActions (o, nil) (rev la)) (old, upds) calls retl ->
+      o = old.
+  Proof.
+    induction la; simpl in *; intros.
+    rewrite (unifyWO retl) in H.
+    inv H; EqDep_subst.
+    inv HRegMapWf.
+    inv H.
+    reflexivity.
+    - unfold compileActions in *; simpl in *.
+      rewrite <- fold_left_rev_right in *.
+      rewrite rev_app_distr, rev_involutive in *; simpl in *.
+      rewrite (unifyWO retl) in H.
+      inv H; simpl in *; EqDep_subst.
+      rewrite (unifyWO WO) in HSemCompActionT_cont.
+      inv HSemCompActionT_cont; simpl in *; EqDep_subst.
+      rewrite (unifyWO val_a0) in HSemCompActionT_a0.
+      inv HSemCompActionT_a0; EqDep_subst.
+      destruct regMap_a.
+      specialize (IHla _ _ _ _ HSemCompActionT_a); subst.
+      destruct regMap_a0.
+      inv HRegMapWf; inv H; inv HSemRegMap.
+      apply (SameOldAction _ _ _ _ (SemVarRegMap _) HSemCompActionT_cont0).
+  Qed.
+
+  Lemma SameOldLoop (m : BaseModule) o:
+    forall rules old upds calls retl,
+      @SemCompActionT Void (compileRules type (o, nil) (rev rules)) (old, upds) calls retl ->
+      o = old.
+  Proof.
+    induction rules; simpl in *; intros.
+    - rewrite (unifyWO retl) in H.
+      inv H; EqDep_subst.
+      inv HRegMapWf.
+      inv H.
+      reflexivity.
+    - unfold compileRules, compileActions in *; simpl in *.
+      rewrite map_app, <- fold_left_rev_right, map_rev in *.
+      simpl in *.
+      rewrite rev_app_distr, rev_involutive in *; simpl in *.
+      rewrite (unifyWO retl) in H.
+      inv H; EqDep_subst.
+      apply Eqdep.EqdepTheory.inj_pair2 in H4; subst; simpl in *.
+      destruct regMap_a.
+      specialize (IHrules _ _ _ _ HSemCompActionT_a); subst.
+      rewrite (unifyWO WO) in HSemCompActionT_cont.
+      inv HSemCompActionT_cont; simpl in *; EqDep_subst.
+      rewrite (unifyWO val_a0) in HSemCompActionT_a0.
+      inv HSemCompActionT_a0; simpl in *; EqDep_subst.
+      destruct regMap_a; inv HRegMapWf; inv H; inv HSemRegMap.
+      apply (SameOldAction _ _ _ _ (SemVarRegMap _) HSemCompActionT_cont0).
+  Qed.
+
+  Lemma PriorityUpdsCompact upds:
+    forall old new,
+      PriorityUpds old upds new -> PriorityUpds old (nil::upds) new.
+  Proof.
+    induction upds.
+    - econstructor 2 with (u := nil) (prevUpds := nil); eauto; repeat constructor.
+      inv H; eauto.
+    - intros.
+      econstructor 2 with (u := nil) (prevUpds := a :: upds); eauto.
+      inv H; auto.
+  Qed.
+
+  Lemma KeyMatch (l1 : RegsT) :
+    NoDup (map fst l1) ->
+    forall l2,
+      map fst l1 = map fst l2 ->
+      (forall s v, In (s, v) l1 -> In (s, v) l2) ->
+      l1 = l2.
+  Proof.
+    induction l1; intros.
+    - destruct l2; inv H0; auto.
+    - destruct a; simpl in *.
+      destruct l2; inv H0.
+      destruct p; simpl in *.
+      inv H.
+      specialize (H1 _ _ (or_introl (eq_refl))) as TMP; destruct TMP.
+      + rewrite H in *.
+        assert (forall s v, In (s, v) l1 -> In (s, v) l2).
+        { intros.
+          destruct (H1 _ _ (or_intror H0)); auto.
+          exfalso.
+          inv H2.
+          apply H3.
+          rewrite in_map_iff.
+          exists (s2, v); auto.
+        }
+        rewrite (IHl1 H5 _ H4 H0).
+        reflexivity.
+      + exfalso.
+        apply H3.
+        rewrite H4, in_map_iff.
+        exists (s, s0); auto.
+  Qed.
+  
+  Lemma PriorityDoubleNil o:
+    NoDup (map fst o) ->
+    forall o',
+      PriorityUpds o (nil::nil) o' ->
+      o = o'.
+  Proof.
+    intros.
+    inv H0; inv HFullU; inv prevCorrect;[|discriminate]; simpl in *.
+    apply getKindAttr_map_fst in currRegsTCurr.
+    assert (forall s v, In (s, v) o' -> In (s, v) prevRegs).
+    { intros.
+      destruct (Hcurr _ _ H0);[contradiction|dest]; auto.
+    }
+    symmetry.
+    apply KeyMatch; auto.
+    rewrite currRegsTCurr in H; assumption.
+  Qed.
+  
+  Lemma CompactPriorityUpds upds:
+    forall old,
+      NoDup (map fst old) ->
+      forall new, 
+        PriorityUpds old (nil::upds) new -> PriorityUpds old upds new.
+  Proof.
+    induction upds; intros.
+    - rewrite (PriorityDoubleNil H H0); constructor.
+    - inv H0; inv HFullU.
+      enough ( new = prevRegs).
+      { rewrite H0; auto. }
+      apply getKindAttr_map_fst in currRegsTCurr.
+      specialize (getKindAttr_map_fst _ _ (prevPrevRegsTrue' prevCorrect)) as P0.
+      rewrite currRegsTCurr in H.
+      eapply KeyMatch; eauto.
+      + rewrite <- currRegsTCurr; assumption.
+      + intros.
+        destruct (Hcurr _ _ H0);[contradiction| dest; auto].
+  Qed.
+
+  Lemma CompactPriorityUpds_iff {old} (NoDupsOld : NoDup (map fst old)) upds new:
+    PriorityUpds old (nil::upds) new <-> PriorityUpds old upds new.
+  Proof.
+    split; eauto using CompactPriorityUpds, PriorityUpdsCompact.
+  Qed.
+  
+  Lemma EquivLoop (m : BaseModule) o:
+    forall rules upds calls retl ls
+           (HoInitNoDups : NoDup (map fst o))
+           (HTrace : Trace m o ls)
+           (HNoMeths : (getMethods m) = nil),
+      SubList rules (getRules m) ->
+      @SemCompActionT Void (compileRules type (o, nil) (rev rules)) (o, upds) calls retl ->
+      (forall u, In u upds -> (NoDup (map fst u)) /\ SubList (getKindAttr u) (getKindAttr o)) /\
+      exists o' (ls' : list (list FullLabel)),
+        PriorityUpds o upds o' /\
+        concat upds = getLabelUpds (concat ls') /\
+        getLabelCalls (concat (rev ls')) = calls /\
+        Trace m o' (ls' ++ ls).
+  Proof.
+    induction rules; simpl in *; intros.
+    - rewrite (unifyWO retl) in H0.
+      inv H0; EqDep_subst.
+      unfold WfRegMapExpr in *; dest.
+      inv H0; split; auto.
+      exists o, nil; repeat split; auto.
+      constructor.
+    - unfold compileRules, compileActions in *; simpl in *.
+      rewrite map_app in *.
+      rewrite <- fold_left_rev_right in *.
+      rewrite map_rev in *.
+      simpl in *.
+      rewrite rev_app_distr in H0.
+      rewrite rev_involutive in *.
+      simpl in *.
+      rewrite (unifyWO retl) in H0.
+      inv H0; simpl in *; EqDep_subst.
+      assert (SubList rules (getRules m)) as P0.
+      { repeat intro; apply H; right; auto. }
+      destruct regMap_a.
+      rewrite (unifyWO WO) in HSemCompActionT_cont.
+      inv HSemCompActionT_cont; simpl in *; EqDep_subst.
+      rewrite (unifyWO val_a0) in HSemCompActionT_a0.
+      inv HSemCompActionT_a0; simpl in *; EqDep_subst.
+      destruct regMap_a.
+      specialize HRegMapWf as HRegMapWf0.
+      inv HRegMapWf; inv H0; inv HSemRegMap.
+      specialize (SameOldAction _ _ _ _ (SemVarRegMap _) HSemCompActionT_cont0) as TMP; subst.
+      specialize (IHrules _ _ _ _ HoInitNoDups HTrace HNoMeths P0 HSemCompActionT_a); dest.
+      rewrite <-CompactPriorityUpds_iff in H2; auto.
+      assert (forall u, In u (nil :: upds0) -> NoDup (map fst u)) as P1.
+      { intros.
+        destruct (H1 _ H7); auto.
+      }
+      assert (WfRegMapExpr (VarRegMap type (o, nil :: upds0)) (o, nil::upds0)) as P2.
+      { clear - HRegMapWf0.
+        unfold WfRegMapExpr in *; dest; split; auto.
+        constructor.
+      }
+      specialize (EquivActions _ HoInitNoDups P1 H2 (eq_sym (prevPrevRegsTrue' H2))
+                               P2 HSemCompActionT_cont0) as TMP; dest.
+      split; auto; simpl in *.
+      assert (upds = (x1::upds0)) as P4.
+      { inv H8.
+        destruct x1; auto.
+      }
+      clear H8; subst.
+      exists (doUpdRegs x1 x), (((x1, (Rle (fst a), calls_cont0))::nil)::x0).
+      unfold getLabelCalls, getLabelUpds in *; simpl in *.
+      rewrite <- H3; simpl in *.
+      repeat split; auto.
+      + econstructor; auto.
+        * rewrite CompactPriorityUpds_iff in H2; auto.
+          apply H2.
+        * specialize (H7 _ (or_introl eq_refl)); dest.
+          rewrite (prevPrevRegsTrue' H2).
+          apply getKindAttr_doUpdRegs; eauto.
+          -- rewrite <- (getKindAttr_map_fst _ _ (prevPrevRegsTrue' H2)).
+             assumption.
+          -- intros.
+             rewrite <- (prevPrevRegsTrue' H2).
+             apply H7.
+             rewrite in_map_iff.
+             exists (s, v); simpl; split; auto.
+        * repeat intro.
+          rewrite (getKindAttr_map_fst _ _ (prevPrevRegsTrue' H2)) in HoInitNoDups.
+          specialize (H7 _ (or_introl eq_refl)); dest.
+          rewrite (prevPrevRegsTrue' H2) in H8.
+          specialize (doUpdRegs_UpdRegs _ (HoInitNoDups) _ H7 H8) as P4.
+          unfold UpdRegs in P4; dest.
+          specialize (H11 _ _ H4); dest.
+          destruct H11; dest.
+          -- inv H11; auto.
+             inv H13.
+          -- right; split; auto.
+             intro; apply H11.
+             exists x1; split; simpl; auto.
+      + repeat rewrite concat_map.
+        repeat rewrite map_app; simpl.
+        repeat rewrite concat_app; simpl.
+        rewrite app_nil_r.
+        reflexivity.
+      + destruct a; simpl in *.
+        econstructor 2.
+        * apply H5.
+        * assert (Step m x ((x1, (Rle s, calls_cont0))::nil)).
+          { econstructor.
+            - econstructor 2; eauto; specialize (Trace_sameRegs HTrace) as TMP; simpl in *.
+              + rewrite <- TMP, (prevPrevRegsTrue' H2); reflexivity.
+              + apply H; left; simpl; reflexivity.
+              + rewrite <- TMP, (prevPrevRegsTrue' H2).
+                apply SubList_map, (SemActionReadsSub H9).
+              + specialize (H7 _ (or_introl eq_refl)); dest.
+                rewrite <- TMP, (prevPrevRegsTrue' H2).
+                apply (SemActionUpdSub H9).
+              + intros; inv H4.
+              + intros; inv H4.
+              + econstructor.
+                rewrite <- TMP.
+                apply (eq_sym (prevPrevRegsTrue' H2)).
+            - unfold MatchingExecCalls_Base; intros.
+              rewrite HNoMeths in H4.
+              inv H4.
+          }
+          apply H4.
+        * simpl.
+          apply doUpdRegs_enuf; auto.
+          -- specialize (H7 _ (or_introl (eq_refl))); dest; auto.
+          -- apply getKindAttr_doUpdRegs; auto.
+             ++ rewrite <-(getKindAttr_map_fst _ _ (prevPrevRegsTrue' H2)); assumption.
+             ++ specialize (H7 _ (or_introl (eq_refl))); dest; assumption.
+             ++ intros.
+                specialize (H7 _ (or_introl (eq_refl))); dest.
+                rewrite <-(prevPrevRegsTrue' H2).
+                apply H8.
+                rewrite in_map_iff.
+                exists (s0, v); auto.
+        * reflexivity.
+  Qed.
+
+End Properties.
